src/riot/RIoT.X509.AliasKeyTBS.fsti
@@ -108,20 +108,19 @@ let valid_aliasKeyTBS_ingredients
   (s_common:  x509_RDN_x520_attribute_string_t COMMON_NAME  IA5_STRING)
   (s_org:     x509_RDN_x520_attribute_string_t ORGANIZATION IA5_STRING)
   (s_country: x509_RDN_x520_attribute_string_t COUNTRY      PRINTABLE_STRING)
-  (ku: key_usage_payload_t)
   (version: datatype_of_asn1_type INTEGER)
 : Type0
-= valid_aliasKeyTBS_extensions_ingredients ku version /\
-  length_of_aliasKeyTBS_extensions ku version
+= valid_aliasKeyTBS_extensions_ingredients version /\
+  v (len_of_aliasKeyTBS_extensions version)
   <= asn1_value_length_max_of_type x509_extensions_outmost_explicit_tag /\
   length_of_x509_version () +
   v (len_of_x509_serialNumber serialNumber) +
   v (len_of_algorithmIdentifier ()) +
-  length_of_aliasKeyTBS_issuer i_common i_org i_country +
+  v (len_of_aliasKeyTBS_issuer i_common i_org i_country) +
   length_of_x509_validity () +
-  length_of_aliasKeyTBS_subject s_common s_org s_country +
+  v (len_of_aliasKeyTBS_subject s_common s_org s_country) +
   length_of_subjectPublicKeyInfo +
-  length_of_x509_extensions (length_of_aliasKeyTBS_extensions ku version)
+  length_of_x509_extensions (v (len_of_aliasKeyTBS_extensions version))
   <= asn1_value_length_max_of_type SEQUENCE
 #pop-options
 
@@ -133,46 +132,31 @@ val lemma_aliasKeyTBS_ingredients_valid
   (s_common:  x509_RDN_x520_attribute_string_t COMMON_NAME  IA5_STRING)
   (s_org:     x509_RDN_x520_attribute_string_t ORGANIZATION IA5_STRING)
   (s_country: x509_RDN_x520_attribute_string_t COUNTRY      PRINTABLE_STRING)
-  (ku: key_usage_payload_t)
   (version: datatype_of_asn1_type INTEGER)
 : Lemma (
   valid_aliasKeyTBS_ingredients
     serialNumber
     i_common i_org i_country
     s_common s_org s_country
-    ku version
+    version
 )
 
 //AR: TODO: 10/03: can we prove lemmas about max lengths of various
 //                 lengths used here, and call those lemmas to help Z3
 //                 prove that their sum is in the range of the return type?
 //                 ditto for the next function
-#push-options "--admit_smt_queries true"
-let length_of_aliasKeyTBS_payload
-  (serialNumber: x509_serialNumber_t)
-  (i_common:  x509_RDN_x520_attribute_string_t COMMON_NAME  IA5_STRING)
-  (i_org:     x509_RDN_x520_attribute_string_t ORGANIZATION IA5_STRING)
-  (i_country: x509_RDN_x520_attribute_string_t COUNTRY      PRINTABLE_STRING)
-  (s_common:  x509_RDN_x520_attribute_string_t COMMON_NAME  IA5_STRING)
-  (s_org:     x509_RDN_x520_attribute_string_t ORGANIZATION IA5_STRING)
-  (s_country: x509_RDN_x520_attribute_string_t COUNTRY      PRINTABLE_STRING)
-  (ku: key_usage_payload_t)
-  (version: datatype_of_asn1_type INTEGER)
-: GTot (asn1_value_length_of_type SEQUENCE)
-= lemma_aliasKeyTBS_extensions_ingredients_valid ku version;
-  lemma_aliasKeyTBS_ingredients_valid
-                serialNumber
-                i_common i_org i_country
-                s_common s_org s_country
-                ku version;
-  length_of_x509_version () +
-  v (len_of_x509_serialNumber serialNumber) +
-  v (len_of_algorithmIdentifier ()) +
-  length_of_aliasKeyTBS_issuer i_common i_org i_country +
-  length_of_x509_validity () +
-  length_of_aliasKeyTBS_subject s_common s_org s_country +
-  length_of_subjectPublicKeyInfo +
-  length_of_x509_extensions (length_of_aliasKeyTBS_extensions ku version)
+// #push-options "--admit_smt_queries true"
+#push-options "--z3rlimit 32"
+let len_of_aliasKeyTBS_payload_max ()
+// : Tot (asn1_value_int32_of_type SEQUENCE)
+= len_of_x509_version () +
+  len_of_x509_serialNumber_max +
+  len_of_algorithmIdentifier () +
+  len_of_aliasKeyTBS_issuer_max () +
+  len_of_x509_validity () +
+  len_of_aliasKeyTBS_subject_max () +
+  len_of_subjectPublicKeyInfo +
+  len_of_x509_extensions (len_of_aliasKeyTBS_extensions_max ())
 
 let len_of_aliasKeyTBS_payload
   (serialNumber: x509_serialNumber_t)
@@ -184,7 +168,7 @@ let len_of_aliasKeyTBS_payload
   (s_country: x509_RDN_x520_attribute_string_t COUNTRY      PRINTABLE_STRING)
   (ku: key_usage_payload_t)
   (version: datatype_of_asn1_type INTEGER)
-: Tot (len: asn1_TLV_int32_of_type SEQUENCE
+: Tot (len: asn1_value_int32_of_type SEQUENCE
             { v len == length_of_aliasKeyTBS_payload
                          serialNumber
                          i_common i_org i_country
@@ -343,7 +327,7 @@ let len_of_aliasKeyTBS
    *
    *     and so, the former does not seem coercible to the latter?
    *)
-  admit ();
+  // admit ();
   len_of_TLV
     (SEQUENCE)
     (len_of_aliasKeyTBS_payload
