src/riot/x509/X509.BasicFields.SerialNumber.fsti
@@ -66,19 +66,28 @@ val lemma_serialize_x509_serialNumber_unfold
  (serialize_big_integer_as_octet_string (v (snd tg)) `serialize` x)
 )
 
-val lemma_serialize_x509_serialNumber_size
+noextract unfold [@@ "opaque_to_smt"]
+let len_of_x509_serialNumber_max = 23ul
+
+let lemma_serialize_x509_serialNumber_size
   (x: x509_serialNumber_t)
 : Lemma (
   length_of_opaque_serialization serialize_x509_serialNumber x ==
-  length_of_big_integer_as_octet_string x
+  v (len_of_big_integer_as_octet_string_TLV x) /\
+  length_of_opaque_serialization serialize_x509_serialNumber x
+  <= v (len_of_x509_serialNumber_max)
 )
+= lemma_serialize_x509_serialNumber_unfold x;
+  lemma_serialize_big_integer_as_octet_string_TLV_unfold x;
+  lemma_serialize_big_integer_as_octet_string_TLV_size x
 
 let len_of_x509_serialNumber
   (x: x509_serialNumber_t)
 : Tot (len: asn1_value_int32_of_big_integer
-            { v len == length_of_opaque_serialization serialize_x509_serialNumber x })
+            { v len == length_of_opaque_serialization serialize_x509_serialNumber x /\
+              v len <= v len_of_x509_serialNumber_max })
 = lemma_serialize_x509_serialNumber_size x;
-  len_of_big_integer_as_octet_string x
+  len_of_big_integer_as_octet_string_TLV x
 
 val serialize32_x509_serialNumber_backwards
 : serializer32_backwards serialize_x509_serialNumber
